Show well-formedness of streams

com.io7m.calino.specification/src/main/coq/Calino/Binary.v
@@ -36,12 +36,40 @@ Inductive streamE : Set :=
   | Vu32 : nat → streamE
   | Vu8  : nat → streamE.
 
-Definition streamSize (s : streamE) : nat :=
+Definition u8byte : byte → streamE :=
+  Vu8 ∘ Byte.to_nat.
+
+Definition streamEIsU8 (e : streamE) : Prop :=
+  match e with
+  | Vu64 _ => False
+  | Vu32 _ => False
+  | Vu8  _ => True
+  end.
+
+Inductive streamWellFormed : list streamE → Prop :=
+  | BEPEmpty : streamWellFormed []
+  | BEPVu64 : ∀ k, 
+      streamWellFormed [Vu64 k]
+  | BEPVu32 : ∀ k, 
+      streamWellFormed [Vu32 k]
+  | BEPVu8s : ∀ es,
+      Forall streamEIsU8 es →
+        length (es) mod 4 = 0 →
+          streamWellFormed es
+  | BEPAppend : ∀ xs ys,
+    streamWellFormed xs →
+      streamWellFormed ys →
+        streamWellFormed (xs ++ ys).
+
+Definition streamElementSize (s : streamE) : nat :=
   match s with
   | Vu64 _ => 8
   | Vu32 _ => 4
   | Vu8  _ => 1
   end.
+
+Definition streamSize (s : list streamE) : nat :=
+  fold_right plus 0 (map streamElementSize s).
 
 Section binaryExpressions.
 
@@ -123,7 +151,7 @@ Section binaryExpressions.
   End binaryExp_ind.
 End binaryExpressions.
 
-Definition sizeMultipleOf (size q : nat) (Hnz : 0 ≠ q) : nat :=
+Definition sizeAsMultipleOf (size q : nat) (Hnz : 0 ≠ q) : nat :=
   let r := size / q in
     match Nat.ltb_spec0 r q with
     | ReflectT _ _ => (r + 1) * q
@@ -132,30 +160,35 @@ Definition sizeMultipleOf (size q : nat) (Hnz : 0 ≠ q) : nat :=
 
 Lemma p0not4 : 0 ≠ 4.
 Proof. discriminate. Qed.
+
 Lemma p0not16 : 0 ≠ 16.
 Proof. discriminate. Qed.
+
+Definition sizeAsMultipleOf4 (size : nat) : nat :=
+  sizeAsMultipleOf size 4 p0not4.
+
+Transparent sizeAsMultipleOf4.
 
 Fixpoint binarySize (b : binaryExp) : nat :=
   match b with
   | BiU32 _     => 4
   | BiU64 _     => 8
-  | BiBytes s   => 4 + sizeMultipleOf (length s) 4 p0not4
-  | BiUTF8 s    => 4 + sizeMultipleOf (length s) 4 p0not4
+  | BiBytes s   => 4 + sizeAsMultipleOf4 (length s)
+  | BiUTF8 s    => 4 + sizeAsMultipleOf4 (length s)
   | BiArray f   => 4 + fold_right plus 0 (map binarySize f)
-  | BiReserve s => sizeMultipleOf s 4 p0not4
+  | BiReserve s => sizeAsMultipleOf4 s
   | BiRecord f  => fold_right plus 0 (map (binarySize ∘ snd) f)
   end.
 
-Definition binaryEvalPaddedBytes 
+Definition binaryEvalPaddedBytes
   (b     : list byte) 
   (align : nat) 
   (Hneq  : 0 ≠ align) 
 : list streamE :=
-  let v8 := map (Vu8 ∘ Byte.to_nat) b in
-  let vm := length v8 mod align in
-    match (Nat.eqb_spec 0 vm) with
-    | ReflectT _ _ => v8
-    | ReflectF _ _ => v8 ++ (repeat (Vu8 0) vm) 
+  let vremaining := length b mod align in
+    match vremaining with
+    | 0 => map u8byte b
+    | _ => map u8byte (b ++ repeat x00 (align - vremaining))
     end.
 
 Fixpoint binaryEval (b : binaryExp) : list streamE :=
@@ -164,13 +197,13 @@ Fixpoint binaryEval (b : binaryExp) : list streamE :=
   | BiU64 k     => [Vu64 k]
   | BiBytes s   => (Vu32 (length s)) :: (binaryEvalPaddedBytes s 4 p0not4)
   | BiUTF8 s    => (Vu32 (length s)) :: (binaryEvalPaddedBytes s 4 p0not4)
-  | BiArray f   => fold_right (@app streamE) [] (map binaryEval f)
-  | BiReserve s => repeat (Vu8 0) (sizeMultipleOf s 4 p0not4)
-  | BiRecord f  => fold_right (@app streamE) [] (map (binaryEval ∘ snd) f)
+  | BiArray f   => (Vu32 (length f)) :: concat (map binaryEval f)
+  | BiReserve s => repeat (Vu8 0) (sizeAsMultipleOf4 s)
+  | BiRecord f  => concat (map (binaryEval ∘ snd) f)
   end.
 
 Definition binarySizePadded16 (b : binaryExp) : nat :=
-  sizeMultipleOf (binarySize b) 16 p0not16.
+  sizeAsMultipleOf (binarySize b) 16 p0not16.
 
 Definition utf8 (s : string) : binaryExp :=
   BiUTF8 (list_byte_of_string s).
@@ -247,10 +280,10 @@ Definition binaryEndSection : binaryExp := BiRecord [
   ("size", u64 0)
 ].
 
-Lemma sizeMultipleOfMod : ∀ s q (Hneq : 0 ≠ q), (sizeMultipleOf s q Hneq) mod q = 0.
+Lemma sizeAsMultipleOfMod : ∀ s q (Hneq : 0 ≠ q), (sizeAsMultipleOf s q Hneq) mod q = 0.
 Proof.
   intros s q Hneq.
-  unfold sizeMultipleOf.
+  unfold sizeAsMultipleOf.
   destruct (Nat.ltb_spec0 (s / q) q) as [Hlt|H1].
   - apply (Nat.mod_mul (s / q + 1) q (Nat.neq_sym _ _ Hneq)).
   - apply (Nat.mod_mul (s / q) q (Nat.neq_sym _ _ Hneq)).
@@ -287,23 +320,25 @@ Proof.
   - reflexivity.
   (* Byte array values are rounded up to a multiple of 4 and prefixed with 4 *)
   - unfold binarySize.
-    remember (sizeMultipleOf (Datatypes.length Hbbyte) 4 p0not4) as size eqn:Heqsize.
+    unfold sizeAsMultipleOf4.
+    remember (sizeAsMultipleOf (Datatypes.length Hbbyte) 4 p0not4) as size eqn:Heqsize.
     rewrite Nat.add_comm.
     rewrite <- (Nat.add_mod_idemp_l size 4 4 (Nat.neq_sym _ _ p0not4)).
     assert (size mod 4 = 0) as Hm0. {
       rewrite Heqsize.
-      apply (sizeMultipleOfMod (Datatypes.length Hbbyte) 4 (p0not4)).
+      apply (sizeAsMultipleOfMod (Datatypes.length Hbbyte) 4 (p0not4)).
     }
     rewrite Hm0.
     reflexivity.
   (* UTF-8 values are rounded up to a multiple of 4 and prefixed with 4 *)
   - unfold binarySize.
-    remember (sizeMultipleOf (Datatypes.length Hbutf) 4 p0not4) as size eqn:Heqsize.
+    unfold sizeAsMultipleOf4.
+    remember (sizeAsMultipleOf (Datatypes.length Hbutf) 4 p0not4) as size eqn:Heqsize.
     rewrite Nat.add_comm.
     rewrite <- (Nat.add_mod_idemp_l size 4 4 (Nat.neq_sym _ _ p0not4)).
     assert (size mod 4 = 0) as Hm0. {
       rewrite Heqsize.
-      apply (sizeMultipleOfMod (Datatypes.length Hbutf) 4 (p0not4)).
+      apply (sizeAsMultipleOfMod (Datatypes.length Hbutf) 4 (p0not4)).
     }
     rewrite Hm0.
     reflexivity.
@@ -325,7 +360,8 @@ Proof.
        apply (divisiblityNAdd 4 (fold_right add 0 (binarySize y :: map binarySize ys)) 4 H0n4 H4mod40 HfoldEq).
   (* Unspecified values are rounded up. *)
   - unfold binarySize.
-    rewrite sizeMultipleOfMod.
+    unfold sizeAsMultipleOf4.
+    rewrite sizeAsMultipleOfMod.
     reflexivity.
   (* Each element of an record is a multiple of 4, so the entire record is too. *)
   - unfold binarySize.
@@ -341,3 +377,311 @@ Proof.
        apply HforAllInd.
        apply (Forall_inv_tail HFF).
 Qed.
+
+Lemma sub_0_lt_ymx : ∀ x y,
+  0 <= x → x < y → 0 < y - x.
+Proof.
+  intros x y Hle Hlt.
+  destruct x as [|a].
+  - rewrite Nat.sub_0_r.
+    exact Hlt.
+  - rewrite <- Nat.lt_add_lt_sub_l.
+    rewrite Nat.add_0_r.
+    exact Hlt.
+Qed.
+
+Lemma mod_sub : ∀ x m,
+  0 < m → 0 < m - (x mod m) <= m.
+Proof.
+  intros x m Hlt.
+  constructor.
+  - assert (0 <= x mod m < m) as HmRange. {
+      apply Nat.mod_bound_pos.
+      apply Nat.le_0_l.
+      exact Hlt.
+    }
+    destruct HmRange as [HA HB].
+    remember (x mod m) as y.
+    apply (sub_0_lt_ymx y m HA HB).
+  - assert (x mod m < m) as HmRange. {
+      apply Nat.mod_upper_bound.
+      apply Nat.neq_sym.
+      apply Nat.lt_neq.
+      exact Hlt.
+    }
+    apply Nat.le_sub_l.
+Qed.
+
+Lemma mod_opposition : ∀ x a,
+  0 ≠ a → x mod a + (a - x mod a) = a.
+Proof.
+  intros x a Hnz.
+  assert (x mod a < a) as Hxma. {
+    apply (Nat.mod_upper_bound).
+    apply Nat.neq_sym.
+    exact Hnz.
+  }
+  remember (x mod a) as y eqn:Heqy.
+  apply Minus.le_plus_minus_r.
+  apply (Nat.lt_le_incl _ _ Hxma).
+Qed.
+
+Theorem binaryEvalPaddedBytesAligned : ∀ bs a (Hnz : 0 ≠ a),
+  length (binaryEvalPaddedBytes bs a Hnz) mod a = 0.
+Proof.
+  intros bs a Hnz.
+  unfold binaryEvalPaddedBytes.
+  destruct (Datatypes.length bs mod a) eqn:Hlen.
+  - rewrite map_length.
+    exact Hlen.
+  - rewrite map_length.
+    rewrite app_length.
+    rewrite repeat_length.
+    rewrite <- Hlen.
+    remember (Datatypes.length bs) as x.
+    rewrite <- (Nat.add_mod_idemp_l x (a - x mod a) a).
+    assert ((x mod a + (a - x mod a)) = a) as Heqa. {
+      rewrite (mod_opposition x a Hnz).
+      reflexivity.
+    }
+    rewrite Heqa.
+    apply Nat.mod_same.
+    apply Nat.neq_sym; exact Hnz.
+    apply Nat.neq_sym; exact Hnz.
+Qed.
+
+Lemma repeat_eq : ∀ (A : Type) (P : A → Prop) (n : nat) (x : A),
+  Forall (eq x) (repeat x n).
+Proof.
+  intros A P n x.
+  induction n as [|m Hm].
+  - constructor.
+  - simpl.
+    constructor.
+    reflexivity.
+    exact Hm.
+Qed.
+
+Lemma Forall_implies : ∀ (A : Type) (P : A → Prop) (Q : A → Prop) (xs : list A) (H : ∀ x, P x → Q x), 
+  Forall P xs → Forall Q xs.
+Proof.
+  intros A P Q xs Ht HforAll.
+  induction HforAll as [|y ys Hpy HfaP HfaQ].
+  - constructor.
+  - constructor.
+    apply (Ht y Hpy).
+    exact HfaQ.
+Qed.
+
+Theorem binaryEvalPaddedBytesU8 : ∀ bs a (Hnz : 0 ≠ a),
+  Forall streamEIsU8 (binaryEvalPaddedBytes bs a Hnz).
+Proof.
+  intros bs a Hnz.
+  unfold binaryEvalPaddedBytes.
+  destruct (Datatypes.length bs mod a) as [|HB].
+  - rewrite Forall_map.
+    induction bs as [|r rs Hrs].
+    -- constructor.
+    -- constructor.
+       reflexivity.
+       exact Hrs.
+  - rewrite map_app.
+    assert (Forall streamEIsU8 (map u8byte bs)) as Hmap. {
+      rewrite Forall_map.
+      induction bs as [|r rs Hrs].
+      - constructor.
+      - constructor.
+        reflexivity.
+        exact Hrs.
+    }
+    assert (Forall streamEIsU8 (map u8byte (repeat "000"%byte (a - S HB)))) as HmapR. {
+      rewrite Forall_map.
+      assert (Forall (eq "000"%byte) (repeat "000"%byte (a - S HB))) as Hfeq
+        by (apply (repeat_eq byte (λ _ : byte, True) (a - S HB) "000"%byte)).
+      simpl.
+      apply (@Forall_implies byte (eq "000"%byte) (λ _ : byte, True) (repeat "000"%byte (a - S HB))). {
+        intros. exact I.
+      }
+      exact Hfeq.
+    }
+    apply Forall_app.
+    constructor.
+    exact Hmap.
+    exact HmapR.
+Qed.
+
+Lemma app_cons : ∀ (A : Type) (x : A) (xs : list A),
+  x :: xs = app (cons x nil) xs.
+Proof.
+  intros A x xs.
+  reflexivity.
+Qed.
+
+Theorem binaryEvalStreamsWellFormed : ∀ b,
+  streamWellFormed (binaryEval b).
+Proof.
+  intros b.
+  induction b as [a0|a1|a2|a3|a4 Hfa|a5|a6 Hfa].
+  (* U32 *)
+  - apply BEPVu32.
+  (* U64 *)
+  - apply BEPVu64.
+  (* Bytes *)
+  - unfold binaryEval.
+    rewrite app_cons.
+    apply BEPAppend.
+    apply BEPVu32.
+    assert (length (binaryEvalPaddedBytes a2 4 p0not4) mod 4 = 0) as Hlm
+      by (apply (binaryEvalPaddedBytesAligned)).
+    apply BEPVu8s.
+    apply binaryEvalPaddedBytesU8.
+    exact Hlm.
+  (* UTF-8 *)
+  - unfold binaryEval.
+    rewrite app_cons.
+    apply BEPAppend.
+    apply BEPVu32.
+    assert (length (binaryEvalPaddedBytes a3 4 p0not4) mod 4 = 0) as Hlm
+      by (apply (binaryEvalPaddedBytesAligned)).
+    assert (Forall streamEIsU8 (binaryEvalPaddedBytes a3 4 p0not4)) as Hu8
+      by (apply (binaryEvalPaddedBytesU8)).
+    apply (BEPVu8s _ Hu8 Hlm).
+  (* Array *)
+  - simpl.
+    rewrite app_cons.
+    apply BEPAppend.
+    apply BEPVu32.
+    induction a4 as [|q qs IHqs].
+    -- constructor.
+    -- assert (streamWellFormed (concat (map binaryEval qs))) as HqsWF
+         by (apply (IHqs (Forall_inv_tail Hfa))).
+       assert (streamWellFormed (binaryEval q)) as HqWF
+         by (apply (Forall_inv Hfa)).
+       simpl.
+       apply BEPAppend.
+       exact HqWF.
+       exact HqsWF.
+  (* Reserve *)
+  - simpl.
+    unfold sizeAsMultipleOf4.
+    remember (sizeAsMultipleOf a5 4 p0not4) as size eqn:Heqsize.
+    assert (size mod 4 = 0) as Heqm. {
+      rewrite Heqsize.
+      apply (sizeAsMultipleOfMod).
+    }
+    assert ((Vu8 ∘ Byte.to_nat) "000"%byte = (Vu8 0)) as HbyteEq by reflexivity.
+    apply BEPVu8s.
+    assert (Forall (eq (Vu8 0)) (repeat (Vu8 0) size)) as Hfeq
+      by (apply (@repeat_eq streamE streamEIsU8 size (Vu8 0))).
+    apply (@Forall_implies streamE (eq (Vu8 0)) streamEIsU8 (repeat (Vu8 0) size)). {
+      intros x Hxeq.
+      unfold streamEIsU8.
+      rewrite <- Hxeq.
+      exact I.
+    }
+    exact Hfeq.
+    rewrite repeat_length.
+    exact Heqm.
+  (* Record *)
+  - simpl.
+    induction a6 as [|q qs IHqs].
+    -- constructor.
+    -- assert (Forall (λ b : binaryExp, streamWellFormed (binaryEval b)) (map snd qs)) as Hfqs. {
+         apply (@Forall_inv_tail binaryExp (λ b : binaryExp, streamWellFormed (binaryEval b)) (snd q) (map snd qs)). {
+           assert ((map snd (q :: qs)) = (snd q :: map snd qs)) as Hmc by reflexivity.
+           rewrite <- Hmc.
+           exact Hfa.
+         }
+       }
+       assert (streamWellFormed (concat (map (binaryEval ∘ snd) qs))) as Hconqs by (apply (IHqs Hfqs)).
+       rewrite map_cons.
+       rewrite concat_cons.
+       apply BEPAppend.
+       rewrite map_cons in Hfa.
+       apply (Forall_inv Hfa).
+       exact Hconqs.
+Qed.
+
+Unset Mangle Names.
+
+Lemma fold_right_1_length : ∀ xs,
+  Forall (eq 1) xs → fold_right add 0 xs = length xs.
+Proof.
+  intros xs Hfa.
+  induction xs as [|y ys IHxs].
+  - reflexivity.
+  - rewrite <- fold_right_add_cons.
+    assert (length (y :: ys) = 1 + length (ys)) as HlenYs by reflexivity.
+    rewrite HlenYs.
+    assert (1 = y) as Hy1 by (apply (Forall_inv Hfa)).
+    rewrite <- Hy1.
+    f_equal.
+    apply IHxs.
+    apply (Forall_inv_tail Hfa).
+Qed.
+
+Theorem fold_right_add_app : ∀ xs ys,
+  fold_right add 0 xs + fold_right add 0 ys = fold_right add 0 (xs ++ ys).
+Proof.
+  intros xs ys.
+  rewrite fold_right_app.
+  generalize dependent ys.
+  induction xs as [|q qs IHqs].
+  - reflexivity.
+  - intros ys.
+    simpl.
+    rewrite <- (IHqs ys).
+    rewrite Nat.add_assoc.
+    reflexivity.
+Qed.
+
+Theorem streamSizeApp : ∀ xs ys,
+  streamSize xs + streamSize ys = streamSize (xs ++ ys).
+Proof.
+  intros xs ys.
+  unfold streamSize.
+  rewrite map_app.
+  rewrite fold_right_add_app.
+  reflexivity.
+Qed.
+
+Theorem streamsWellFormedDivisible4 : ∀ es,
+  streamWellFormed es → streamSize es mod 4 = 0.
+Proof.
+  intros es Hwf.
+  induction Hwf as [|H1|H2|es Hfa Hsize|xs ys Hxswf Hxsize Hyswf Hysize].
+  - reflexivity.
+  - reflexivity.
+  - reflexivity.
+  - unfold streamSize.
+    assert (Forall (λ e, 1 = streamElementSize e) es) as HFaSize. { 
+      apply (@Forall_implies streamE streamEIsU8 (λ e : streamE, 1 = streamElementSize e) es). {
+        intros x His.
+        destruct x as [u64|u32|u8].
+        - contradiction.
+        - contradiction.
+        - reflexivity.
+      }
+      exact Hfa.
+    }
+    assert (Forall (eq 1) (map streamElementSize es)) as Hall1. {
+      apply (@Forall_map _ _ _ _ es).
+      exact HFaSize.
+    }
+    assert (fold_right add 0 (map streamElementSize es) = length es) as HlenEq. {
+      assert (length es = length (map streamElementSize es)) as HmapLen. {
+        rewrite map_length.
+        reflexivity.
+      }
+      rewrite HmapLen.
+      apply (fold_right_1_length (map streamElementSize es) Hall1).
+    }
+    rewrite HlenEq.
+    exact Hsize.
+  - rewrite <- streamSizeApp.
+    apply divisiblityNAdd.
+    discriminate.
+    exact Hxsize.
+    exact Hysize.
+Qed.
+
